wip: labels_equiv_position_in proof

theories/common/LanguagesCommon.v
@@ -26,6 +26,37 @@ Definition eqb_lbl l1 l2 :=
   end.
 
 
+Definition eqb_opt_lbl opt_label opt_label' :=
+  match opt_label with 
+  | Some lbl => match opt_label' with
+                | Some lbl' => eqb_lbl lbl lbl'
+                | None => false
+                end
+  | None => false
+  end.
+
+
+Lemma bool_symm : forall n m, (n =? m) = (m =? n).
+Proof.
+  induction n; destruct m; auto.
+  simpl. auto.
+Qed.
+
+Theorem eqb_lbl_symm : forall x y, eqb_lbl x y = eqb_lbl y x.
+Proof.
+  destruct x; destruct y; auto.
+  simpl. apply bool_symm.
+Qed.
+
+
+
+
+Lemma eqb_opt_lbl_symm : forall opt opt',
+  eqb_opt_lbl opt opt' = eqb_opt_lbl opt' opt.
+Proof.
+  induction opt; destruct opt'; auto.
+  simpl. apply eqb_lbl_symm.
+Qed.
 
 Theorem eqb_lbl_refl : forall v, eqb_lbl v v = true.
 Proof.
@@ -37,11 +68,7 @@ Proof.
   destruct v; try (apply PeanoNat.Nat.eqb_refl); reflexivity.
 Qed.
 
-Lemma bool_symm : forall n m, (n =? m) = (m =? n).
-Proof.
-  induction n; destruct m; auto.
-  simpl. auto.
-Qed.
+
 
 
 Theorem eqb_var_symm : forall x y, eqb_var x y = eqb_var y x.
@@ -89,3 +116,4 @@ Proof.
   - apply var_eqb_eq in Heq. left. assumption.
   - apply var_eqb_neq in Heq. right. assumption.
 Qed.
+
