theories/nat_lang/NatLang.v
@@ -135,9 +135,8 @@ Definition create_state x :=
 
 
 Definition eq_inst_label (instr : instruction ) (opt_lbl : option label) :=
-  match instr, opt_lbl with 
-  | Instr (Some lbl_a) _, Some lbl_b => eqb_lbl lbl_a lbl_b
-  | _, _                => false
+  match instr with 
+  | Instr opt_lbl' _ => eqb_opt_lbl opt_lbl' opt_lbl
   end.
 
 (** Função para encontrar a posição da primeira instrução com certa label 
